type safety for adjusted extension and elem definitions

theories/operations.v
@@ -516,21 +516,26 @@ Definition stab_elem (s: store_record) (inst: instance) (x: N) (i: nat) : option
   | _ => None
   end.
 
-Definition tab_update (tab : tableinst) (i : nat) (tabv: value_ref) : tableinst :=
-  {| tableinst_type := tab.(tableinst_type);
-     tableinst_elem := set_nth tabv tab.(tableinst_elem) i tabv |}.
+Definition tab_update (tab : tableinst) (i : nat) (tabv: value_ref) : option tableinst :=
+  if (Nat.ltb i (tab_size tab)) then
+    if (tab.(tableinst_type).(tt_elem_type) == typeof_ref tabv) then
+      Some {| tableinst_type := tab.(tableinst_type);
+        tableinst_elem := set_nth tabv tab.(tableinst_elem) i tabv |}
+    else None
+  else None.
 
 Definition stab_update (s: store_record) (inst: instance) (x: N) (i: nat) (tabv: value_ref) : option store_record :=
   match lookup_N inst.(inst_tables) x with
   | Some tabaddr => 
       match lookup_N s.(s_tables) tabaddr with
       | Some tab =>
-          if (Nat.ltb i (tab_size tab)) then
-          let: tab' := tab_update tab i tabv in
-          let: tabs' := set_nth tab' s.(s_tables) (N.to_nat tabaddr) tab' in
-            Some (Build_store_record (s_funcs s) tabs' (s_mems s)
-                    (s_globals s) (s_elems s) (s_datas s))
-          else None
+          match tab_update tab i tabv with
+          | Some tab' =>
+              let: tabs' := set_nth tab' s.(s_tables) (N.to_nat tabaddr) tab' in
+              Some (Build_store_record (s_funcs s) tabs' (s_mems s)
+                      (s_globals s) (s_elems s) (s_datas s))
+          | None => None
+          end
       | None => None
       end
   | _ => None
